more poggers

rollup.v
@@ -7,7 +7,7 @@ From stdpp Require Import gmap.
 From stdpp Require Import mapset.
 From stdpp Require Import sets.
 From stdpp Require Import list.
-Import gmap_utils.
+Require Import gmap_utils.
 
 Section stuff.
 
@@ -25,7 +25,7 @@ Class TPCM (M : Type) `{EqDecision M} :=
   assoc : forall x y z , dot x (dot y z) = dot (dot x y) z ;
   reflex : forall x , mov x x ;
   trans : forall x y z , mov x y -> mov y z -> mov x z ;
-  mov_monotonic : forall x y z ,
+  mov_onotonic : forall x y z ,
       mov x y -> valid (dot x z) -> valid (dot y z) /\ mov (dot x z) (dot y z)
 }.
 
@@ -117,6 +117,18 @@ Definition cell_total (cell: Cell) (lifetime: Lifetime) :=
   match cell with
   | CellCon m _ _ reserved => dot m (sum_reserved_over_lifetime reserved lifetime)
   end.
+  
+Definition rel_project `{TPCM R, TPCM M} (ref : Refinement R M) (r: R) :=
+    match (rel R M ref) r with | Some t => t | None => unit end.
+
+Definition get_ref (ri: option RefinementIndex) : Refinement M M. Admitted.
+ 
+Definition project (node: Node) (m: M) : M :=
+  match node with
+  | CellNode (CellCon _ ref _ _) _ => rel_project (get_ref ref) m
+  | FailNode => unit
+  end
+.
 
 Fixpoint node_total (node: Node) (lifetime: Lifetime) : M :=
   match node with
@@ -126,10 +138,10 @@ Fixpoint node_total (node: Node) (lifetime: Lifetime) : M :=
 with branch_total (branch: Branch) (lifetime: Lifetime) : M :=
   match branch with
   | BranchNil => unit
-  | BranchCons _ node branch => dot (project (node_total node lifetime)) (branch_total branch lifetime)
+  | BranchCons _ node branch => dot (project node (node_total node lifetime)) (branch_total branch lifetime)
   end
 .
-
+ 
 Definition umbrella : M -> (M -> Prop) := tpcm_le.
 
 Definition umbrella_unit : (M -> Prop) := λ _ , True.
@@ -143,6 +155,8 @@ Definition conjoin_umbrella (a b : (M -> Prop)) : (M -> Prop) :=
 Definition project_umbrella
     (refinement: Refinement M M) (umbrella : M -> Prop) : (M -> Prop) :=
     λ m , ∃ r t , umbrella r /\ (rel M M refinement r = Some t) /\ tpcm_le t m.
+
+Definition umbrella_is_closed (umb: M -> Prop) := ∀ a b , umb a -> umb (dot a b).
     
 Definition conjoin_reserved_over_lifetime (reserved: gmap nat M) (lifetime: Lifetime) : (M -> Prop) :=
   set_fold (λ lu um , conjoin_umbrella um (umbrella (gmap_get_or_unit reserved lu)))
@@ -153,6 +167,16 @@ Definition cell_view (cell: Cell) (lifetime: Lifetime) : (M -> Prop) :=
   | CellCon m _ _ reserved => conjoin_reserved_over_lifetime reserved lifetime
   end.
 
+Definition rel_project_fancy (ref : Refinement M M) (um: M -> Prop) :=
+    λ x , ∃ a b , tpcm_le a x /\ rel M M ref b = Some a /\ um b.
+  
+Definition project_fancy (node: Node) (um: M -> Prop) : (M -> Prop) :=
+  match node with
+  | CellNode (CellCon _ ref _ _) _ => rel_project_fancy (get_ref ref) um
+  | FailNode => umbrella_unit
+  end
+.
+
 Fixpoint node_view (node: Node) (lifetime: Lifetime) : (M -> Prop) :=
   match node with
   | CellNode cell branch => conjoin_umbrella (cell_view cell lifetime) (branch_view branch lifetime)
@@ -161,32 +185,228 @@ Fixpoint node_view (node: Node) (lifetime: Lifetime) : (M -> Prop) :=
 with branch_view (branch: Branch) (lifetime: Lifetime) : (M -> Prop) :=
   match branch with
   | BranchNil => umbrella_unit
-  | BranchCons _ node branch => conjoin_umbrella (node_view node lifetime) (branch_view branch lifetime)
+  | BranchCons _ node branch => conjoin_umbrella (project_fancy node (node_view node lifetime)) (branch_view branch lifetime)
   end
 .
 
 Definition view_sat (umbrella : M -> Prop) (m : M) := umbrella m.
 
+Lemma self_le_self a : tpcm_le a a.
+Proof. unfold tpcm_le. exists unit. rewrite unit_dot. trivial. Qed.
+
+Lemma unit_view_sat_unit : view_sat umbrella_unit unit.
+Proof. unfold view_sat. unfold umbrella_unit. trivial. Qed.
+
+Lemma le_add_both_sides a b c : tpcm_le a b -> tpcm_le (dot a c) (dot b c).
+Proof.  unfold tpcm_le. intros. destruct H0. exists x. rewrite comm. rewrite assoc.
+    rewrite comm in H0. rewrite H0. trivial. Qed.
+    
+Lemma le_add_right_side a b c : tpcm_le a b -> tpcm_le a (dot b c).
+Proof.  unfold tpcm_le. intros. destruct H0. exists (dot x c). rewrite assoc.
+    rewrite H0. trivial. Qed.
+
+Lemma umbrella_closed_umbrella_unit : umbrella_is_closed umbrella_unit.
+Proof. unfold umbrella_is_closed. unfold umbrella_unit. intros. trivial. Qed.
+
+Lemma umbrella_closed_umbrella a : umbrella_is_closed (umbrella a).
+Proof. unfold umbrella_is_closed. unfold umbrella. intros. apply le_add_right_side. trivial.
+Qed.
+
+Lemma umbrella_closed_conjoin um1 um2 : umbrella_is_closed um1 -> umbrella_is_closed um2 ->
+    umbrella_is_closed (conjoin_umbrella um1 um2).
+Proof. unfold umbrella_is_closed. unfold conjoin_umbrella. intros.
+  destruct H2. destruct H2. destruct H2. destruct H3. exists x. exists (dot x0 b). split.
+    - trivial.
+    - split.
+      + apply H1. trivial.
+      + rewrite <- H4. apply assoc.
+Qed.
+
 Lemma sum_reserved_over_lifetime_monotonic (g: gmap nat M) (lt1: Lifetime) (lt2: Lifetime)
   (lt1_le_lt2 : subseteq lt1 lt2)
   : tpcm_le
         (sum_reserved_over_lifetime g lt1)
-        (sum_reserved_over_lifetime g lt2). Admitted.
+        (sum_reserved_over_lifetime g lt2).
+Proof. unfold sum_reserved_over_lifetime.
+  unfold Lifetime in lt1, lt2.
+  apply (gset_subset_relate tpcm_le).
+  - apply self_le_self.
+  - trivial.
+  - intros. apply le_add_both_sides. trivial.
+  - intros. apply le_add_right_side. trivial.
+  - intros. rewrite <- assoc. rewrite <- assoc. f_equal. apply comm.
+Qed.
 
 Lemma view_sat_reserved_over_lifetime (g: gmap nat M) (lt: Lifetime)
   : view_sat (conjoin_reserved_over_lifetime g lt)
-             (sum_reserved_over_lifetime g lt). Admitted.
+             (sum_reserved_over_lifetime g lt).
+Proof.
+  unfold conjoin_reserved_over_lifetime, sum_reserved_over_lifetime.
+  apply (gset_relate view_sat).
+  - apply unit_view_sat_unit.
+  - intros. unfold view_sat in *. unfold conjoin_umbrella.
+      exists c. exists (gmap_get_or_unit g a). repeat split.
+    + trivial.
+    + unfold umbrella. apply self_le_self.
+Qed.
 
+Lemma view_sat_with_le (umb: M -> Prop) (a : M) (b : M)
+    (closed: umbrella_is_closed umb)
+    (vs: view_sat umb a)
+    (mle: tpcm_le a b) : view_sat umb b.
+Proof. unfold view_sat in *. intros. unfold umbrella_is_closed in closed.
+    unfold tpcm_le in mle. destruct mle. rewrite <- H0. apply closed. trivial.
+Qed.
+
+Lemma conjoin_reserved_over_lifetime_is_closed (reserved: gmap nat M) (lt: Lifetime)
+    : umbrella_is_closed (conjoin_reserved_over_lifetime reserved lt).
+Proof. unfold cell_view. unfold conjoin_reserved_over_lifetime.
+  apply (gset_easy_induct umbrella_is_closed).
+  - apply umbrella_closed_umbrella_unit.
+  - intros. apply umbrella_closed_conjoin.
+    + trivial.
+    + apply umbrella_closed_umbrella.
+Qed.
 
 Lemma cell_view_le_total (cell: Cell) (lt: Lifetime) (active: Lifetime)
     (lt_is_active : lifetime_included active lt)
     : view_sat (cell_view cell lt) (cell_total cell active).
 Proof.
   unfold cell_view. destruct cell. unfold cell_total.
-    have sub : subseteq lt active.
-       - unfold lifetime_included in lt_is_active. trivial.
-  - have ineq1 := sum_reserved_over_lifetime_monotonic g lt active sub.
-    have ineq2 := view_sat_reserved_over_lifetime g lt.
+    apply view_sat_with_le with (a := (sum_reserved_over_lifetime g lt)).
+    + apply conjoin_reserved_over_lifetime_is_closed.
+    + apply view_sat_reserved_over_lifetime.
+    + rewrite comm. apply le_add_right_side.
+        apply sum_reserved_over_lifetime_monotonic.
+        unfold lifetime_included in lt_is_active. trivial.
+Qed.
 
+Lemma view_sat_conjoin (um1 um2 : M -> Prop) (m1 m2 : M)
+    (vs1: view_sat um1 m1)
+    (vs2: view_sat um2 m2)
+    : view_sat (conjoin_umbrella um1 um2) (dot m1 m2).
+Proof. unfold view_sat in *. unfold conjoin_umbrella. exists m1. exists m2. repeat split; trivial. Qed.
 
+Definition in_refinement_domain (ref: Refinement M M) (m : M) :=
+  match rel M M ref m with | Some _ => True | None => False end.
+
+Fixpoint node_all_total_in_refinement_domain (node: Node) (lifetime: Lifetime) : Prop :=
+  match node with
+  | CellNode (CellCon _ ref _ _) branch =>
+         in_refinement_domain (get_ref ref) (node_total node lifetime)
+      /\ branch_all_total_in_refinement_domain branch lifetime
+  | FailNode => false
+  end
+with branch_all_total_in_refinement_domain (branch: Branch) (lifetime: Lifetime) : Prop :=
+  match branch with
+  | BranchNil => True
+  | BranchCons _ node branch =>
+         node_all_total_in_refinement_domain node lifetime
+      /\ branch_all_total_in_refinement_domain branch lifetime
+  end
+.
+
+Definition view_sat_projections (ref: Refinement M M) (view : M -> Prop) (m : M)
+    (vrv : in_refinement_domain ref m)
+    (vs: view_sat view m)
+      : view_sat
+        (rel_project_fancy ref view) (*(node_view (CellNode (CellCon m o b0 g) b) lt))*)
+        (rel_project       ref m). (*(node_total (CellNode (CellCon m o b0 g) b) active))*)
+Proof. 
+  unfold rel_project_fancy. unfold rel_project. unfold view_sat. unfold tpcm_le.
+  exists (match rel M M ref m with | Some t => t | None => unit end).
+  exists m.
+  repeat split.
+  - exists unit. apply unit_dot.
+  - unfold in_refinement_domain in vrv. destruct (rel M M ref m).
+    + trivial.
+    + contradiction.
+  - unfold view_sat in vs. trivial.
+Qed.
+
+Lemma node_view_le_total (node: Node) (lt: Lifetime) (active: Lifetime)
+    (lt_is_active : lifetime_included active lt)
+    (ird: node_all_total_in_refinement_domain node active)
+    : view_sat (node_view node lt) (node_total node active)
+with branch_view_le_total (branch: Branch) (lt: Lifetime) (active: Lifetime)
+    (lt_is_active : lifetime_included active lt)
+    (ird: branch_all_total_in_refinement_domain branch active)
+    : view_sat (branch_view branch lt) (branch_total branch active).
+Proof.
+ - destruct node.
+      + unfold node_view. unfold node_total. apply view_sat_conjoin.
+        * apply cell_view_le_total. trivial.
+        * apply branch_view_le_total; trivial.
+          unfold node_all_total_in_refinement_domain in ird.
+              fold branch_all_total_in_refinement_domain in ird.
+              destruct c in ird. destruct ird. trivial.
+      + unfold node_view. unfold node_total. apply unit_view_sat_unit.
+ - destruct branch.
+      + unfold branch_view. unfold branch_total. apply view_sat_conjoin.
+        * fold node_view. fold node_total.
+            unfold project_fancy. unfold project.
+            (* instantiate inductive hypotheses here, so the prover can 
+               infer decreasing arguments *)
+            have ind_node := node_view_le_total n0. clear node_view_le_total.
+            have ind_branch := branch_view_le_total branch. clear branch_view_le_total.
+            destruct n0.
+          -- destruct c. apply view_sat_projections.
+              ++ unfold branch_all_total_in_refinement_domain in ird. destruct ird.
+                  destruct H0. trivial.
+              ++ apply ind_node; trivial. 
+                  unfold branch_all_total_in_refinement_domain in ird. crush.
+          -- apply unit_view_sat_unit.
+        * apply branch_view_le_total; trivial.
+            unfold branch_all_total_in_refinement_domain in ird. crush.
+      + unfold view_sat, branch_view, branch_total. unfold umbrella_unit. trivial.
+Qed.
+
+Definition cell_trivial (cell: Cell) :=
+  match cell with
+  | CellCon m _ borrows reserves => (∀ b , borrows b = false) /\ reserves = empty /\ m = unit
+  end
+.
+
+Fixpoint node_trivial (node: Node) :=
+  match node with
+  | CellNode cell branch => cell_trivial cell /\ branch_trivial branch
+  | FailNode => False
+  end
+with branch_trivial (branch: Branch) :=
+  match branch with
+  | BranchNil => True
+  | BranchCons _ node branch => node_trivial node /\ branch_trivial branch
+  end
+.
+
+Fixpoint node_equiv (node1: Node) (node2: Node) :=
+  match node1, node2 with
+    | FailNode, FailNode => True
+    | FailNode, CellNode _ _ => False
+    | CellNode _ _, FailNode => False
+    | CellNode cell1 branch1, CellNode cell2 branch2 =>
+           cell1 = cell2
+        /\ branch_equiv branch1 branch2
+  end
+with branch_equiv (branch1: Branch) : Branch -> Prop :=
+  fix inner_branch_equiv (branch2: Branch) :=
+    match branch1 with
+      | BranchNil => branch_trivial branch2
+      | BranchCons id1 n1 br1 =>
+          match branch2 with
+          | BranchNil => branch_trivial branch1
+          | BranchCons id2 n2 br2 =>
+               ((id1 = id2) /\ node_equiv n1 n2 /\ branch_equiv br1 br2)
+            \/ (node_trivial n1 /\ branch_equiv br1 branch2)
+            \/ (node_trivial n2 /\ inner_branch_equiv br2)
+          end
+    end
+.
+
+Instance inst_node_equiv : Equiv Node := node_equiv.
+
+Inductive State :=
+  | StateCon : Lifetime -> Node -> State
+  | StateFail
+.
 
